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Abstract

Projection of a point (x̂, ŷ, ẑ) onto the exponential cone {x, y, z|y exp(x/y) ≤ z, y ≥ 0}
is a fundamental atomic operation used in conic optimization. The open-source solver SCS
implemented such a projection via an ad-hoc iterative algorithm proj exp cone which was
later incorporated and adapted into diffcp under the name proj exp cone. The resulting
code is compact and elegant, but, because I couldn’t find a note explaining the algorithm,
I ended up writing this short note to give an overview of its inner mechanics1.

1 One problem, multiple formulations

For a given point (x̂, ŷ, ẑ), finding its exponential cone projection consists in solving an equality
constrained least squares problem2:

min
x,y,z

1

2
((x− x̂)2 − (y − ŷ)2 − (z − ẑ)2)

s.t. y exp(x/y) = z

The Lagrangian of this optimization problem is

1

2
((x− x̂)2 − ((y − ŷ)2 − (z − ẑ)2) + µ(y exp(x/y)− z) (1)

where µ is the dual variable of the constraint y exp(x/y) = z. The KKT condition at the solution
(x∗, y∗, z∗, µ∗) are

x∗ − x̂+ µ∗ exp(x∗/y∗) = 0 (2)

y∗ − ŷ + µ∗ exp(x∗/y∗)(1− x∗/y∗) = 0 (3)

z∗ − ẑ − µ∗ = 0 (4)

y∗ exp(x∗/y∗)− z∗ = 0 (5)

An equivalent formulation to the original minimization problem is

min
x,y,z

1

2
((x− x̂)2 − (y − ŷ)2 − (z − ẑ)2)

s.t. x+ y log(y/z) = 0

1I have tried to keep the names of the variables in the formulas as close as possible to the name of the variables
in the C++ code. Known parameters are in blue .

2We have supposed that (x̂, ŷ, ẑ) is strictly outside the exponential cone.

1

https://www.cvxgrp.org/scs/
https://github.com/cvxgrp/scs/blob/eee0cca45655540a4207acaab17379763cf59867/src/cones.c
https://github.com/cvxgrp/diffcp
https://github.com/cvxgrp/diffcp/blob/master/cpp/src/cones.cpp


2 SOLVING THE ρ-FORMULATION 2

The Lagrangian of this optimization problem is

1

2
((x− x̂)2 − ((y − ŷ)2 − (z − ẑ)2) + ρ(x+ y log(y/z)) (6)

where ρ is the dual variable of the constraint x + y log(y/z) = 0. The KKT condition at the
solution (x∗, y∗, z∗, µ∗) are

x∗ − x̂+ ρ∗ = 0 (7)

y∗ − ŷ + ρ∗(log(y∗/z∗) + 1) = 0 (8)

z∗ − ẑ − ρ∗y∗/z∗ = 0 (9)

x∗ + y∗ log(y∗/z∗) = 0 (10)

2 Solving the ρ-formulation

We start with a few algebraic manipulations:

� Equation 7 implies

x∗ = x̂− ρ∗ (11)

� Equation 9 implies
y∗ = ẑ(z∗ − ẑ)/ρ∗ (12)

� Replacing y∗ in (8) by (12) gives

z∗(z∗ − ẑ)

ρ∗2
− ŷ

ρ
+ log(

z∗ − ẑ

ρ∗
) + 1 = 0 (13)

which is equivalent to
(t∗ + ẑ)t∗

ρ∗2
− ŷ

ρ
+ log(

t∗

ρ∗
) + 1 = 0 (14)

where t∗ := z∗ − ẑ.

For a given value of ρ∗, the system of equations 11, 12 and 13 can be solved in the following
order

1. Find t∗ by solving (14) via a 1-dimensional Newton method.

2. Set z∗ := t∗ + ẑ (which solves equation 13).

3. Set y∗ = ẑ(z∗ − ẑ)/ρ∗ (which is equation 12).

4. Set x∗ = x̂− ρ∗ (which is equation 11).

The above equations explicitly show us how the 3 first equations of the KKT system (7, 8,
9) express (x∗, y∗, z∗) as a function of ρ∗.

In order to identify all four parameters (x∗, y∗, z∗, ρ∗), we have now to use the fourth equation
of the KKT system (10). This is performed via a bisection algorithm, which returns ρ∗ such that
x∗(ρ∗) + y∗(ρ∗) log(y∗(ρ∗)/z∗(ρ∗)) = 0
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